@prefix dsv:      <https://w3id.org/dsv-ontology#> .
@prefix owl:      <http://www.w3.org/2002/07/owl#> .
@prefix xsd:      <http://www.w3.org/2001/XMLSchema#> .
@prefix rdfs:     <http://www.w3.org/2000/01/rdf-schema#> .
@prefix rdf:      <http://www.w3.org/1999/02/22-rdf-syntax-ns#> .
@prefix dc:       <http://purl.org/dc/elements/1.1/> .
@prefix vann:     <http://purl.org/vocab/vann/> .
@prefix dcterms:  <http://purl.org/dc/terms/> .
@prefix foaf:     <http://xmlns.com/foaf/0.1/> .
@prefix csvw:     <http://www.w3.org/ns/csvw#> .
@prefix qb:       <http://purl.org/linked-data/cube#> .

###########################################
# DataSet-Variable Ontology
###########################################

<https://w3id.org/dsv-ontology#> a owl:Ontology;
  rdfs:comment "Ontology for describing relationships between datasets and variables."@en,
    "Ontology for describing relationships between datasets and variables.";
  rdfs:label "DataSet-Variable Ontology"@en, "DataSet-Variable Ontology.";
  dc:contributor "The DataSet-Variable Ontology is part of the work of the ODISSEI project, funded by the Netherlands Organisation of Scientific Research (NWO), ODISSEI Roadmap project: 184.035.014."@en;
  dc:creator "Margherita Martorana"@en, "Tobias Kuhn"@en, "Ronald Siebes"@en, "Jacco van Ossenbruggen"@en;
  dc:rights "The DataSet-Variable Ontology Ontology is available under the Creative Commons Attribution 4.0 license; see http://creativecommons.org/licenses/by/4.0/."@en;
  dc:subject "Dataset, Variable"@en;
  dc:title "The DataSet-Variable Ontology"@en;
  dcterms:license <http://creativecommons.org/licenses/by/4.0/>;
  vann:preferredNamespacePrefix "dsv";
  vann:preferredNamespaceUri "https://w3id.org/dsv-ontology#";
  owl:versionInfo "V1.0 - 2023 Release"@en;
  foaf:homepage <https://w3id.org/dsv-ontology> .

###########################################
# Classes
###########################################

<https://w3id.org/dsv-ontology#Dataset> a owl:Class;
  rdfs:subClassOf qb:DataSet, csvw:Table;
  rdfs:comment "Set of data.";
  rdfs:label "Dataset" .

<https://w3id.org/dsv-ontology#AggregatedDataset> a owl:Class;
  rdfs:subClassOf <https://w3id.org/dsv-ontology#Dataset>;
  rdfs:comment "Set of data that has been aggregated over an individual - or unaggregated - set of data.";
  rdfs:label "Aggregated Dataset" .

<https://w3id.org/dsv-ontology#IndividualDataset> a owl:Class;
  rdfs:subClassOf <https://w3id.org/dsv-ontology#Dataset>;
  rdfs:comment "Set of data that can be aggregated over. Usually representing the raw data. ";
  rdfs:label "Individual Dataset" .

<https://w3id.org/dsv-ontology#DatasetSchema> a owl:Class;
  rdfs:subClassOf qb:DataStructureDefinition, csvw:TableSchema;
  rdfs:comment "The structural schema of a dataset.";
  rdfs:label "Dataset Schema" .

<https://w3id.org/dsv-ontology#DatasetComponent> a owl:Class;
  rdfs:subClassOf qb:ComponentSpecification;
  rdfs:comment "Set of individual component of a dataset.";
  rdfs:label "Dataset Component" .

<https://w3id.org/dsv-ontology#Variable> a owl:Class;
  rdfs:comment "The variable described by a component of the dataset.";
  rdfs:label "Variable" .

<https://w3id.org/dsv-ontology#SummaryStatistics> a owl:Class;
  rdfs:comment "Set of summary statistics about the dataset or column.";
  rdfs:label "Summary Statistics" .

<https://w3id.org/dsv-ontology#StatisticalDataType> a owl:Class;
  rdfs:comment "Set of statistical data types.";
  rdfs:label "Statistical Data Type" .

<https://w3id.org/dsv-ontology#QualitativeStatisticalDataType> a owl:Class;
  rdfs:subClassOf <https://w3id.org/dsv-ontology#StatisticalDataType>;
  rdfs:comment "Set of statistical data types can be observed and - or - categorised.";
  rdfs:label "Qualitative Statistical Data Type" .

<https://w3id.org/dsv-ontology#NominalStatisticalDataType> a owl:Class;
  rdfs:subClassOf <https://w3id.org/dsv-ontology#QualitativeStatisticalDataType>;
  rdfs:comment "Statistical data type representing discrete units that cannot be ordered or measured.";
  rdfs:label "Nominal Statistical Data Type" .

<https://w3id.org/dsv-ontology#OrdinalStatisticalDataType> a owl:Class;
  rdfs:subClassOf <https://w3id.org/dsv-ontology#QualitativeStatisticalDataType>;
  rdfs:comment "Statistical data type representing discrete units that can be ordered or measured.";
  rdfs:label "Ordinal Statistical Data Type" .

<https://w3id.org/dsv-ontology#QuantitativeStatisticalDataType> a owl:Class;
  rdfs:subClassOf <https://w3id.org/dsv-ontology#StatisticalDataType>;
  rdfs:comment "Set of statistical data types can be measured and quantified.";
  rdfs:label "Quantitative Statistical Data Type" .

<https://w3id.org/dsv-ontology#IntervalStatisticalDataType> a owl:Class;
  rdfs:subClassOf <https://w3id.org/dsv-ontology#QuantitativeStatisticalDataType>;
  rdfs:comment "Statistical data type representing ordered data measured over a numerical scale with equal distance between units.";
  rdfs:label "Interval Statistical Data Type" .

<https://w3id.org/dsv-ontology#RatioStatisticalDataType> a owl:Class;
  rdfs:subClassOf <https://w3id.org/dsv-ontology#QuantitativeStatisticalDataType>;
  rdfs:comment "Statistical data type representing ordered data with equal distance between units, where negative values are not allowed.";
  rdfs:label "Ratio Statistical Data Type" .


###########################################
# Object Properties
###########################################                  

<https://w3id.org/dsv-ontology#datasetSchema> a owl:ObjectProperty;
  rdfs:subPropertyOf qb:structure, csvw:tableSchema;
  rdfs:domain <https://w3id.org/dsv-ontology#Dataset>;
  rdfs:range <https://w3id.org/dsv-ontology#DatasetSchema>;
  rdfs:comment "Property linking the dataset to its schema.";
  rdfs:label "dataset schema" .

<https://w3id.org/dsv-ontology#datasetComponent> a owl:ObjectProperty;
  rdfs:subPropertyOf qb:component;
  rdfs:domain <https://w3id.org/dsv-ontology#DatasetSchema>;
  rdfs:range <https://w3id.org/dsv-ontology#DatasetComponent>;
  rdfs:comment "Property linking the dataset schema to its components.";
  rdfs:label "dataset component" .

<https://w3id.org/dsv-ontology#componentProperty> a owl:ObjectProperty;
  rdfs:subPropertyOf qb:dimension, csvw:propertyUrl;
  rdfs:domain <https://w3id.org/dsv-ontology#DatasetComponent>;
  rdfs:range rdf:Property;
  rdfs:comment "Property linking a component to a property.";
  rdfs:label "component property" .

<https://w3id.org/dsv-ontology#refersToVariable> a owl:ObjectProperty;
  rdfs:domain <https://w3id.org/dsv-ontology#DatasetComponent>;
  rdfs:range <https://w3id.org/dsv-ontology#Variable>;
  rdfs:comment "Property linking a component to a variable.";
  rdfs:label "refers to variable" .

<https://w3id.org/dsv-ontology#linksToVariable> a owl:ObjectProperty;
  rdfs:domain rdf:Property;
  rdfs:range <https://w3id.org/dsv-ontology#Variable>;
  rdfs:comment "Property linking a property of a component to a variable.";
  rdfs:label "links to variable" .

<https://w3id.org/dsv-ontology#subVariableOf> a owl:ObjectProperty;
  rdfs:domain <https://w3id.org/dsv-ontology#Variable>;
  rdfs:range <https://w3id.org/dsv-ontology#Variable>;
  rdfs:comment "Property linking a variable to its sub-variable.";
  rdfs:label "sub-variable of" .

<https://w3id.org/dsv-ontology#rowsRepresentInstancesOf> a owl:ObjectProperty;
  rdfs:domain <https://w3id.org/dsv-ontology#Dataset>;
  rdfs:range owl:Class;
  rdfs:comment "Property linking a dataset to the conceptual representation of its rows.";
  rdfs:label "rows represent instances of" .

<https://w3id.org/dsv-ontology#summaryStatistics> a owl:ObjectProperty;
  rdfs:domain <https://w3id.org/dsv-ontology#Dataset>, <https://w3id.org/dsv-ontology#DatasetComponent>;
  rdfs:range <https://w3id.org/dsv-ontology#SummaryStatistics>;
  rdfs:comment "Property linking a dataset or a component to their summary statistics.";
  rdfs:label "summary statistics" .

<https://w3id.org/dsv-ontology#statisticalDataType> a owl:ObjectProperty;
  rdfs:domain <https://w3id.org/dsv-ontology#SummaryStatistics>;
  rdfs:range <https://w3id.org/dsv-ontology#StatisticalDataType>;
  rdfs:comment "Property linking a component to its statistical data type.";
  rdfs:label "statistical data type" .

###########################################
# Data Properties
###########################################   

<https://w3id.org/dsv-ontology#numberOfColumns> a owl:DataProperty;
  rdfs:domain <https://w3id.org/dsv-ontology#SummaryStatistics>;
  rdfs:range xsd:integer;
  rdfs:comment "Property linking a dataset or a component to their summary statistics.";
  rdfs:label "number of columns" .

<https://w3id.org/dsv-ontology#numberOfRows> a owl:DataProperty;
  rdfs:domain <https://w3id.org/dsv-ontology#SummaryStatistics>;
  rdfs:range xsd:integer;
  rdfs:comment "Property linking a dataset or a component to their summary statistics.";
  rdfs:label "number of rows" .

<https://w3id.org/dsv-ontology#completeness> a owl:DataProperty;
  rdfs:domain <https://w3id.org/dsv-ontology#SummaryStatistics>;
  rdfs:range xsd:float;
  rdfs:comment "Property linking a dataset or a component to their summary statistics.";
  rdfs:label "completeness" .

dsv:statisticalDataType             a                   owl:DataProperty ;
                                    rdfs:domain         dsv:SummaryStatistics ;
                                    rdfs:range          xsd:string . 

<https://w3id.org/dsv-ontology#missingValueFormat> a owl:DataProperty;
  rdfs:domain <https://w3id.org/dsv-ontology#SummaryStatistics>;
  rdfs:range xsd:string;
  rdfs:comment "Property linking a dataset or a component to their summary statistics.";
  rdfs:label "missing value format" .
